hiccupSum with chk

boogie_examples/hiccupSum.bpl
@@ -1,5 +1,7 @@
 /* Simple example of data-dependent alignment. 
-   Depends on havoc'd choices rather than input. */
+   Depends on havoc'd choices rather than input. 
+   Could verify with lockstep but then it's not an example of data dependent.
+*/
 
 procedure hiccupSum (n: int) returns (r: int)
 { var h: bool; var i: int;  
@@ -17,21 +19,56 @@ procedure hiccupSum_eq (n, n': int) returns (r, r': int)
   i, r := 0, 0;   i', r' := 0, 0;
   havoc h; havoc h';
 
-  while (i < n || i' < n') // left/right alignment conditions h/h'
+  while (i < n || i' < n') // left/right alignment conditions h and (!h && h')
     invariant i == i';  
-    invariant r == r'; 
+    invariant r == r';
+    invariant (i < n && i' < n') || (i >= n && i' >= n') || (i < n && h) || (i' < n' && (!h && h'));
     { 
-      if (h && i < n) { // left body only 
+      if (h && i < n) { // left only 
         if (!h) { r := r+i; i := i+1; } havoc h;
-      } else if (h' && i' < n') { // right body only 
-        if (!h') { r' := r'+i'; i' := i'+1; } havoc h';
-      } else if (i < n && i' < n' && !h && !h') { // both 
+      } else if (!h && h' && i' < n') { // right only 
+        if (!h') { r' := r'+i'; i' := i'+1; } havoc h'; assume !h'; 
+      } else if (i < n && i' < n' && !h && !(!h && h')) { // both 
         if (!h) { r := r+i; i := i+1; } havoc h;
-        if (!h') { r' := r'+i'; i' := i'+1; } havoc h';
+        if (!h') { r' := r'+i'; i' := i'+1; } havoc h'; // no need for filter?
       } else {
         assert false; // adequacy condition
       }       
    }
 }
 
+function bool2int(x:bool):int { if x then 1 else 0 } 
+
+procedure hiccupSum_eq_chk (n, n': int) returns (r, r': int)
+  requires n == n';   ensures r == r';                     
+{ 
+  var h, h': bool; var i, i': int; 
+  var vsnap: int; var rosnap: bool;
+  i, r := 0, 0;   i', r' := 0, 0;
+  havoc h; havoc h';
+
+  while (i < n || i' < n') // left/right alignment conditions h and (!h && h')
+    invariant i == i';    // variant: bool2int(h')
+    invariant r == r';
+    invariant (i < n && i' < n') || (i >= n && i' >= n') || (i < n && h) || (i' < n' && (!h && h'));
+    { 
+      vsnap := bool2int(h'); // added by chk
+      rosnap := i' < n' && !h && h'; // added by chk 
+      if (h && i < n) { // left only 
+        if (!h) { r := r+i; i := i+1; } havoc h;
+      } else if (!h && h' && i' < n') { // right only 
+        if (!h') { r' := r'+i'; i' := i'+1; } 
+        assert (exists v:bool :: v == !h'); // added by chk
+        havoc h'; assume (!h'); 
+      } else if (i < n && i' < n' && !h && !(!h && h')) { // both 
+        if (!h) { r := r+i; i := i+1; } havoc h;
+        if (!h') { r' := r'+i'; i' := i'+1; } 
+        havoc h'; // no filter needed 
+      } else {
+        assert false; // adequacy condition
+      }       
+      assert rosnap ==> 0 <= bool2int(h');
+      assert rosnap ==> bool2int(h') < vsnap;
+   }
+}
           
